src/Init/Data/Nat/Linear.lean
@@ -170,21 +170,7 @@ structure PolyCnstr  where
   eq  : Bool
   lhs : Poly
   rhs : Poly
-  deriving BEq
-
--- TODO: implement LawfulBEq generator companion for BEq
-instance : LawfulBEq PolyCnstr where
-  eq_of_beq {a b} h := by
-    cases a; rename_i eq₁ lhs₁ rhs₁
-    cases b; rename_i eq₂ lhs₂ rhs₂
-    have h : eq₁ == eq₂ && lhs₁ == lhs₂ && rhs₁ == rhs₂ := h
-    simp at h
-    have ⟨⟨h₁, h₂⟩, h₃⟩ := h
-    rw [h₁, h₂, h₃]
-  rfl {a} := by
-    cases a; rename_i eq lhs rhs
-    show (eq == eq && lhs == lhs && rhs == rhs) = true
-    simp [LawfulBEq.rfl]
+  deriving DecidableEq
 
 def PolyCnstr.mul (k : Nat) (c : PolyCnstr) : PolyCnstr :=
   { c with lhs := c.lhs.mul k, rhs := c.rhs.mul k }
