tests/lean/1079.lean
@@ -1,13 +1,13 @@
 theorem bad : ∀ (m n : Nat), (if m = n then Ordering.eq else Ordering.gt) = Ordering.lt → False := by
   intros m n
-  cases (Nat.decEq m n) with -- an error as expected: "alternative `isFalse` has not bee provided"
+  cases (decEq m n) with -- an error as expected: "alternative `isFalse` has not bee provided"
   | isTrue h =>
     set_option trace.Meta.Tactic.simp true in
     simp [h]
 
 theorem bad' : ∀ (m n : Nat), (if m = n then Ordering.eq else Ordering.gt) = Ordering.lt → False := by
   intros m n
-  cases (Nat.decEq m n) with
+  cases (decEq m n) with
   | isTrue h =>
     simp [h]
   | isFalse h =>
