tests/lean/run/1311.lean
@@ -1,7 +1,5 @@
-instance : DecidableEq ByteArray
-  | ⟨a⟩, ⟨b⟩ => match decEq a b with
-    | isTrue h₁  => isTrue $ congrArg ByteArray.mk h₁
-    | isFalse h₂ => isFalse $ fun h => by cases h; cases (h₂ rfl)
+instance : DecidableEq ByteArray :=
+  .ofInj (fun ⟨a⟩ => a) @fun ⟨a⟩ ⟨b⟩ h => by simp_all
 
 #eval ByteArray.empty = ByteArray.empty
 #eval ByteArray.empty != ByteArray.empty.push 5
